feat(KSA): System Key (#1021) (#1055)
Co-authored-by: José Corella <39066999+josecorella@users.noreply.github.com>

AwsCryptographicMaterialProviders/runtimes/java/src/examples/java/software/amazon/cryptography/example/hierarchy/mutations/MutationsProvider.java
@@ -1,0 +1,171 @@
+package software.amazon.cryptography.example.hierarchy.mutations;
+
+import java.util.Collections;
+import java.util.HashMap;
+import java.util.List;
+import java.util.stream.Collectors;
+import javax.annotation.Nonnull;
+import javax.annotation.Nullable;
+import software.amazon.awssdk.services.kms.KmsClient;
+import software.amazon.cryptography.example.hierarchy.AdminProvider;
+import software.amazon.cryptography.keystore.model.AwsKms;
+import software.amazon.cryptography.keystoreadmin.KeyStoreAdmin;
+import software.amazon.cryptography.keystoreadmin.model.ApplyMutationInput;
+import software.amazon.cryptography.keystoreadmin.model.ApplyMutationOutput;
+import software.amazon.cryptography.keystoreadmin.model.ApplyMutationResult;
+import software.amazon.cryptography.keystoreadmin.model.InitializeMutationInput;
+import software.amazon.cryptography.keystoreadmin.model.InitializeMutationOutput;
+import software.amazon.cryptography.keystoreadmin.model.KeyManagementStrategy;
+import software.amazon.cryptography.keystoreadmin.model.KmsSymmetricEncryption;
+import software.amazon.cryptography.keystoreadmin.model.KmsSymmetricKeyArn;
+import software.amazon.cryptography.keystoreadmin.model.MutatedBranchKeyItem;
+import software.amazon.cryptography.keystoreadmin.model.MutationToken;
+import software.amazon.cryptography.keystoreadmin.model.Mutations;
+import software.amazon.cryptography.keystoreadmin.model.SystemKey;
+import software.amazon.cryptography.keystoreadmin.model.TrustStorage;
+
+public class MutationsProvider {
+
+  public static String mutatedItemsToString(
+    List<MutatedBranchKeyItem> mutatedItems
+  ) {
+    return mutatedItems
+      .stream()
+      .map(item -> String.format("%s : %s", item.ItemType(), item.Description())
+      )
+      .collect(Collectors.joining(",\n"));
+  }
+
+  public static Mutations defaultMutation(
+    @Nonnull final String terminalKmsArn
+  ) {
+    HashMap<String, String> terminalEC = new HashMap<>(2, 1);
+    terminalEC.put("Robbie", "is a dog.");
+    return Mutations
+      .builder()
+      .TerminalEncryptionContext(terminalEC)
+      .TerminalKmsArn(terminalKmsArn)
+      .build();
+  }
+
+  public static SystemKey KmsSystemKey(@Nonnull final String systemKeyArn) {
+    return KmsSystemKey(systemKeyArn, null, null);
+  }
+
+  public static SystemKey KmsSystemKey(
+    @Nonnull final String systemKeyArn,
+    @Nullable KmsClient systemKeyKmsClient,
+    @Nullable List<String> systemKeyGrantTokens
+  ) {
+    //noinspection unchecked
+    final List<String> tempList = systemKeyGrantTokens == null
+      ? Collections.EMPTY_LIST
+      : systemKeyGrantTokens;
+    final KmsClient tempKms = systemKeyKmsClient == null
+      ? AdminProvider.kms(null)
+      : systemKeyKmsClient;
+    final AwsKms tempAws = AwsKms
+      .builder()
+      .kmsClient(tempKms)
+      .grantTokens(tempList)
+      .build();
+    return SystemKey
+      .builder()
+      .kmsSymmetricEncryption(
+        KmsSymmetricEncryption
+          .builder()
+          .AwsKms(tempAws)
+          .KmsArn(KmsSymmetricKeyArn.builder().KmsKeyArn(systemKeyArn).build())
+          .build()
+      )
+      .build();
+  }
+
+  public static SystemKey TrustStorage() {
+    return SystemKey
+      .builder()
+      .trustStorage(TrustStorage.builder().build())
+      .build();
+  }
+
+  public static void workMutation(
+    String branchKeyId,
+    SystemKey systemKey,
+    MutationToken token,
+    KeyManagementStrategy strategy,
+    KeyStoreAdmin admin
+  ) {
+    boolean done = false;
+    int limitLoop = 10;
+
+    while (!done) {
+      ApplyMutationResult result = workPage(
+        branchKeyId,
+        systemKey,
+        token,
+        strategy,
+        admin,
+        1
+      );
+
+      if (result.ContinueMutation() != null) {
+        token = result.ContinueMutation();
+      }
+      if (result.CompleteMutation() != null) {
+        done = true;
+      }
+      if (limitLoop == 0) {
+        done = true;
+      }
+      limitLoop--;
+    }
+  }
+
+  static ApplyMutationResult workPage(
+    String branchKeyId,
+    SystemKey systemKey,
+    MutationToken token,
+    KeyManagementStrategy strategy,
+    KeyStoreAdmin admin,
+    Integer pageSize
+  ) {
+    ApplyMutationInput applyInput = ApplyMutationInput
+      .builder()
+      .MutationToken(token)
+      .PageSize(pageSize)
+      .Strategy(strategy)
+      .SystemKey(systemKey)
+      .build();
+    ApplyMutationOutput applyOutput = admin.ApplyMutation(applyInput);
+    ApplyMutationResult result = applyOutput.MutationResult();
+
+    System.out.println(
+      "ApplyLogs: " +
+      branchKeyId +
+      " items: \n" +
+      mutatedItemsToString(applyOutput.MutatedBranchKeyItems())
+    );
+    return result;
+  }
+
+  static MutationToken executeInitialize(
+    String branchKeyId,
+    KeyStoreAdmin admin,
+    InitializeMutationInput initInput,
+    String logPrefix
+  ) {
+    InitializeMutationOutput initOutput = admin.InitializeMutation(initInput);
+    MutationToken token = initOutput.MutationToken();
+    System.out.println(
+      logPrefix +
+      ": " +
+      "\nFlag: " +
+      initOutput.InitializeMutationFlag().toString() +
+      "\nIdentifier: " +
+      branchKeyId +
+      "\nitems: \n" +
+      mutatedItemsToString(initOutput.MutatedBranchKeyItems())
+    );
+    return token;
+  }
+}
