AwsCryptographicMaterialProviders/runtimes/java/src/testExamples/java/software/amazon/cryptography/example/hierarchy/mutations/TestMutationsSystemKeyKMSTamper.java
@@ -1,0 +1,271 @@
+package software.amazon.cryptography.example.hierarchy.mutations;
+
+import static software.amazon.cryptography.example.hierarchy.mutations.MutationsProvider.executeInitialize;
+import static software.amazon.cryptography.example.hierarchy.mutations.MutationsProvider.workPage;
+
+import java.nio.charset.StandardCharsets;
+import java.util.Collections;
+import java.util.HashMap;
+import java.util.Map;
+import java.util.Objects;
+import org.testng.Assert;
+import org.testng.annotations.Test;
+import software.amazon.awssdk.core.SdkBytes;
+import software.amazon.awssdk.services.dynamodb.model.AttributeAction;
+import software.amazon.awssdk.services.dynamodb.model.AttributeValue;
+import software.amazon.awssdk.services.dynamodb.model.AttributeValueUpdate;
+import software.amazon.cryptography.example.Fixtures;
+import software.amazon.cryptography.example.hierarchy.AdminProvider;
+import software.amazon.cryptography.example.hierarchy.CreateKeyExample;
+import software.amazon.cryptography.example.hierarchy.StorageExample;
+import software.amazon.cryptography.keystore.KeyStorageInterface;
+import software.amazon.cryptography.keystoreadmin.KeyStoreAdmin;
+import software.amazon.cryptography.keystoreadmin.model.InitializeMutationInput;
+import software.amazon.cryptography.keystoreadmin.model.KeyManagementStrategy;
+import software.amazon.cryptography.keystoreadmin.model.MutationToken;
+import software.amazon.cryptography.keystoreadmin.model.MutationVerificationException;
+import software.amazon.cryptography.keystoreadmin.model.Mutations;
+import software.amazon.cryptography.keystoreadmin.model.SystemKey;
+
+public class TestMutationsSystemKeyKMSTamper {
+
+  static final String testPrefix = "java-test-mutation-system-key-kms-tamper-";
+
+  public static Map<String, AttributeValue> ddbKeyForCommitment(
+    final String identifier
+  ) {
+    Map<String, AttributeValue> ddbKey = new HashMap<>(3, 1);
+    ddbKey.put("branch-key-id", AttributeValue.fromS(identifier));
+    ddbKey.put("type", AttributeValue.fromS("branch:MUTATION_COMMITMENT"));
+    return ddbKey;
+  }
+
+  public static Map<String, AttributeValue> ddbKeyForIndex(
+    final String identifier
+  ) {
+    Map<String, AttributeValue> ddbKey = new HashMap<>(3, 1);
+    ddbKey.put("branch-key-id", AttributeValue.fromS(identifier));
+    ddbKey.put("type", AttributeValue.fromS("branch:MUTATION_INDEX"));
+    return ddbKey;
+  }
+
+  @Test
+  public void testCreateTimeCommitment() {
+    Map<String, AttributeValueUpdate> tamper = new HashMap<>(2, 1);
+    tamper.put(
+      "create-time",
+      AttributeValueUpdate
+        .builder()
+        .value(AttributeValue.fromS("now!"))
+        .action(AttributeAction.PUT)
+        .build()
+    );
+    testAttribute(
+      tamper,
+      testPrefix + "create-time-commitment-",
+      "branch:MUTATION_COMMITMENT"
+    );
+  }
+
+  @Test
+  public void testCreateTimeIndex() {
+    Map<String, AttributeValueUpdate> tamper = new HashMap<>(2, 1);
+    tamper.put(
+      "create-time",
+      AttributeValueUpdate
+        .builder()
+        .value(AttributeValue.fromS("now!"))
+        .action(AttributeAction.PUT)
+        .build()
+    );
+    testAttribute(
+      tamper,
+      testPrefix + "create-time-index-",
+      "branch:MUTATION_INDEX"
+    );
+  }
+
+  // Tampering the H-Version results in a Key Storage Failure
+  // @Test
+  // public void testHierarchyVersion() {
+  //   Map<String, AttributeValueUpdate> tamper = new HashMap<>(2, 1);
+  //   tamper.put(
+  //     "hierarchy-version",
+  //     AttributeValueUpdate
+  //       .builder()
+  //       .value(AttributeValue.fromN("2"))
+  //       .action(AttributeAction.PUT)
+  //       .build()
+  //   );
+  //   testAttribute(tamper, testPrefix + "hierarchy-version-");
+  // }
+
+  @Test
+  public void testInput() {
+    Map<String, AttributeValueUpdate> tamper = new HashMap<>(2, 1);
+    tamper.put(
+      "input",
+      AttributeValueUpdate
+        .builder()
+        .value(
+          AttributeValue.fromB(
+            SdkBytes.fromString(
+              "{\"kms-arn\":\"arn:aws:kms:us-west-2:658956600833:key/mrk-80bd8ecdcd4342aebd84b7dc9da498a7\"}",
+              StandardCharsets.UTF_8
+            )
+          )
+        )
+        .action(AttributeAction.PUT)
+        .build()
+    );
+    testAttribute(tamper, testPrefix + "input-", "branch:MUTATION_COMMITMENT");
+  }
+
+  @Test
+  public void testOriginal() {
+    Map<String, AttributeValueUpdate> tamper = new HashMap<>(2, 1);
+    tamper.put(
+      "original",
+      AttributeValueUpdate
+        .builder()
+        .value(
+          AttributeValue.fromB(
+            SdkBytes.fromString(
+              "{\"kms-arn\":\"arn:aws:kms:us-west-2:658956600833:key/mrk-80bd8ecdcd4342aebd84b7dc9da498a7\"}",
+              StandardCharsets.UTF_8
+            )
+          )
+        )
+        .action(AttributeAction.PUT)
+        .build()
+    );
+    testAttribute(
+      tamper,
+      testPrefix + "original-",
+      "branch:MUTATION_COMMITMENT"
+    );
+  }
+
+  @Test
+  public void testTerminal() {
+    Map<String, AttributeValueUpdate> tamper = new HashMap<>(2, 1);
+    tamper.put(
+      "terminal",
+      AttributeValueUpdate
+        .builder()
+        .value(
+          AttributeValue.fromB(
+            SdkBytes.fromString(
+              "{\"kms-arn\":\"arn:aws:kms:us-west-2:658956600833:key/mrk-80bd8ecdcd4342aebd84b7dc9da498a7\"}",
+              StandardCharsets.UTF_8
+            )
+          )
+        )
+        .action(AttributeAction.PUT)
+        .build()
+    );
+    testAttribute(
+      tamper,
+      testPrefix + "terminal-",
+      "branch:MUTATION_COMMITMENT"
+    );
+  }
+
+  @Test
+  public void testPageIndex() {
+    Map<String, AttributeValueUpdate> tamper = new HashMap<>(2, 1);
+    tamper.put(
+      "pageIndex",
+      AttributeValueUpdate
+        .builder()
+        .value(
+          AttributeValue.fromB(
+            SdkBytes.fromString("Done", StandardCharsets.UTF_8)
+          )
+        )
+        .action(AttributeAction.PUT)
+        .build()
+    );
+    testAttribute(tamper, testPrefix + "pageIndex-", "branch:MUTATION_INDEX");
+  }
+
+  public void testAttribute(
+    Map<String, AttributeValueUpdate> tamper,
+    String testPrefix,
+    String type
+  ) {
+    final String identifier =
+      testPrefix + java.util.UUID.randomUUID().toString();
+
+    CreateKeyExample.CreateKey(
+      Fixtures.TEST_KEYSTORE_NAME,
+      Fixtures.TEST_LOGICAL_KEYSTORE_NAME,
+      Fixtures.MRK_ARN_WEST,
+      identifier,
+      Fixtures.ddbClientWest2
+    );
+    //noinspection unchecked
+    SystemKey systemKey = MutationsProvider.KmsSystemKey(
+      Fixtures.POSTAL_HORN_KEY_ARN,
+      Fixtures.kmsClientWest2,
+      Collections.EMPTY_LIST
+    );
+    KeyStoreAdmin admin = AdminProvider.admin(
+      Fixtures.TEST_KEYSTORE_NAME,
+      Fixtures.TEST_LOGICAL_KEYSTORE_NAME,
+      Fixtures.ddbClientWest2
+    );
+    Mutations mutations = MutationsProvider.defaultMutation(
+      Fixtures.POSTAL_HORN_KEY_ARN
+    );
+    KeyManagementStrategy strategy = AdminProvider.strategy(null);
+    InitializeMutationInput initInput = InitializeMutationInput
+      .builder()
+      .Mutations(mutations)
+      .Identifier(identifier)
+      .Strategy(strategy)
+      .SystemKey(systemKey)
+      .build();
+    MutationToken token = executeInitialize(
+      identifier,
+      admin,
+      initInput,
+      "InitLogs"
+    );
+    Map<String, AttributeValue> ddbKey = Objects.equals(
+        type,
+        "branch:MUTATION_COMMITMENT"
+      )
+      ? ddbKeyForCommitment(identifier)
+      : ddbKeyForIndex(identifier);
+    Fixtures.ddbClientWest2.updateItem(builder ->
+      builder
+        .attributeUpdates(tamper)
+        .tableName(Fixtures.TEST_KEYSTORE_NAME)
+        .key(ddbKey)
+    );
+    boolean exThrown = false;
+    try {
+      workPage(identifier, systemKey, token, strategy, admin, 1);
+    } catch (MutationVerificationException ex) {
+      System.out.println(
+        "Apply with wrong SystemKey failed with: \n" +
+        ex.getClass().getSimpleName() +
+        ": " +
+        ex.getMessage()
+      );
+      exThrown = true;
+    }
+    KeyStorageInterface storage = StorageExample.create(
+      Fixtures.ddbClientWest2,
+      Fixtures.TEST_KEYSTORE_NAME,
+      Fixtures.TEST_LOGICAL_KEYSTORE_NAME
+    );
+    Assert.assertTrue(
+      exThrown,
+      "Tampering should have lead to a MutationVerificationException! testId: " +
+      identifier
+    );
+    Fixtures.cleanUpBranchKeyId(storage, identifier);
+  }
+}
