AwsCryptographicMaterialProviders/dafny/AwsCryptographyKeyStoreAdmin/test/SystemKey/TestInitializeMutation.dfy
@@ -1,0 +1,135 @@
+// Copyright Amazon.com Inc. or its affiliates. All Rights Reserved.
+// SPDX-License-Identifier: Apache-2.0
+
+include "../../src/Index.dfy"
+include "../../../AwsCryptographyKeyStore/test/CleanupItems.dfy"
+include "../../../AwsCryptographyKeyStore/test/Fixtures.dfy"
+include "../AdminFixtures.dfy"
+
+// Tests that Initialize Mutation with a System Key of Trust Storage:
+// - Will FAKE Sign Commitment and Index
+// - Will FAKE Validate Commitment and Index on second call
+// - Will FAIL Validate if ciphertext blob is not "trustStorage"
+
+// Tests that Initialize Mutation with a System Key of KMS:
+// - Will Sign Commitment and Index
+// - Will Validate Commitment and Index on second call
+
+module {:options "/functionSyntax:4" } TestSystemKey.TestInitializeMutation {
+  import Types = AwsCryptographyKeyStoreAdminTypes
+  import KeyStoreAdmin
+  import KeyStore
+  import KeyStoreTypes = AwsCryptographyKeyStoreTypes
+  import opened Wrappers
+  import Fixtures
+  import AdminFixtures
+  import UUID
+  import CleanupItems
+  import KMS = Com.Amazonaws.Kms
+  import DDB = Com.Amazonaws.Dynamodb
+  import DefaultKeyStorageInterface
+  import Time
+  import Structure
+  import String = StandardLibrary.String
+  import UTF8
+
+  const happyCaseId := "test-mutate-kms-arn-only"
+  const customEC := "aws-crypto-ec:Robbie"
+  const kmsId: string := Fixtures.keyArn
+  const physicalName: string := Fixtures.branchKeyStoreName
+  const logicalName: string := Fixtures.logicalKeyStoreName
+
+  const trustStorageHPrefix := "\nTestSystemKey.TestInitializeMutation :: TrustStorageHappyCase :: "
+  const trustStorageHCaseId := "dafny-system-key-test-initialize-mutation-trust-storage-happy-case"
+  method {:test} TrustStorageHappyCase()
+  {
+    var kmsClient :- expect Fixtures.ProvideKMSClient();
+    var underTest :- expect AdminFixtures.DefaultAdmin();
+    var strategy :- expect AdminFixtures.DefaultKeyManagerStrategy(kmsClient?:=Some(kmsClient));
+    var systemKey := Some(Types.SystemKey.trustStorage(trustStorage := Types.TrustStorage()));
+    var uuid :- expect UUID.GenerateUUID();
+    var testId := trustStorageHCaseId + "-" + uuid;
+    Fixtures.CreateHappyCaseId(id:=testId);
+
+    var mutationsRequest := Types.Mutations(TerminalKmsArn := Some(Fixtures.postalHornKeyArn));
+    var initInput := Types.InitializeMutationInput(
+      Identifier := testId,
+      Mutations := mutationsRequest,
+      Strategy := Some(strategy),
+      SystemKey := systemKey,
+      DoNotVersion := Some(false));
+    var initializeOutput :- expect underTest.InitializeMutation(initInput);
+    var initializeToken := initializeOutput.MutationToken;
+
+    var initializeAgainOutput :- expect underTest.InitializeMutation(initInput);
+    expect initializeToken == initializeAgainOutput.MutationToken;
+
+    var kmSystemKey := Types.SystemKey.kmsSymmetricEncryption(
+      kmsSymmetricEncryption := Types.KmsSymmetricEncryption(
+        KmsArn := Types.KmsKeyArn(Fixtures.publicKeyArn),
+        AwsKms := KeyStoreTypes.AwsKms(
+          grantTokens := None,
+          kmsClient := Some(kmsClient))));
+
+    var sadInput := Types.InitializeMutationInput(
+      Identifier := testId,
+      Mutations := mutationsRequest,
+      Strategy := Some(strategy),
+      SystemKey := Some(kmSystemKey),
+      DoNotVersion := Some(false));
+
+    var sadOutput := underTest.InitializeMutation(sadInput);
+    // TODO Restore this last expectation.
+    expect sadOutput.Failure?, "Should have failed to initialize.";
+
+    var ddbClient :- expect Fixtures.ProvideDDBClient();
+    var _ := CleanupItems.DeleteBranchKeyWithOneVersion(testId, ddbClient);
+  }
+
+  const kmsSymEncHPrefix := "\nTestSystemKey.TestInitializeMutation :: KmsSymEncHappyCase :: "
+  const kmsSymEncHCaseId := "dafny-system-key-test-initialize-mutation-kmsSymEnc-happy-case"
+  method {:test} KmsSymEncHappyCase()
+  {
+    var kmsClient :- expect Fixtures.ProvideKMSClient();
+    var underTest :- expect AdminFixtures.DefaultAdmin();
+    var strategy :- expect AdminFixtures.DefaultKeyManagerStrategy(kmsClient?:=Some(kmsClient));
+    var kmSystemKey := Types.SystemKey.kmsSymmetricEncryption(
+      kmsSymmetricEncryption := Types.KmsSymmetricEncryption(
+        KmsArn := Types.KmsKeyArn(Fixtures.publicKeyArn),
+        AwsKms := KeyStoreTypes.AwsKms(
+          grantTokens := None,
+          kmsClient := Some(kmsClient))));
+    var uuid :- expect UUID.GenerateUUID();
+    var testId := trustStorageHCaseId + "-" + uuid;
+    Fixtures.CreateHappyCaseId(id:=testId);
+
+    var mutationsRequest := Types.Mutations(TerminalKmsArn := Some(Fixtures.postalHornKeyArn));
+    var initInput := Types.InitializeMutationInput(
+      Identifier := testId,
+      Mutations := mutationsRequest,
+      Strategy := Some(strategy),
+      SystemKey := Some(kmSystemKey),
+      DoNotVersion := Some(false));
+    var initializeOutput :- expect underTest.InitializeMutation(initInput);
+    var initializeToken := initializeOutput.MutationToken;
+
+    var initializeAgainOutput :- expect underTest.InitializeMutation(initInput);
+    expect initializeToken == initializeAgainOutput.MutationToken;
+
+    var trustSK := Some(Types.SystemKey.trustStorage(trustStorage := Types.TrustStorage()));
+    var sadInput := Types.InitializeMutationInput(
+      Identifier := testId,
+      Mutations := mutationsRequest,
+      Strategy := Some(strategy),
+      SystemKey := trustSK,
+      DoNotVersion := Some(false));
+
+    var sadOutput := underTest.InitializeMutation(sadInput);
+    // TODO Restore this last expectation.
+    expect sadOutput.Failure?, "Should have failed to initialize.";
+
+    var ddbClient :- expect Fixtures.ProvideDDBClient();
+    var _ := CleanupItems.DeleteBranchKeyWithOneVersion(testId, ddbClient);
+  }
+
+}
